Dataflow/WellFormed/Decide.v
@@ -3,12 +3,14 @@ Require Import Rustre.Dataflow.Syntax.
 Require Import Rustre.Dataflow.IsFree.
 Require Import Rustre.Dataflow.IsFree.Decide.
 Require Import Rustre.Dataflow.IsVariable.
+Require Import Rustre.Dataflow.IsVariable.Decide.
 Require Import Rustre.Dataflow.IsDefined.
+Require Import Rustre.Dataflow.IsDefined.Decide.
 Require Import Rustre.Dataflow.WellFormed.
 
 (** * Well formed CoreDF programs: decision procedure *)
 
-(** 
+(**
 
 Decision procedure for the [Is_well_sch] predicate. We show that it is
 equivalent to its specification.
@@ -21,8 +23,6 @@ Remark: This development is not formally part of the correctness proof.
 Section Decide.
 
 Variable mems : PS.t.
-
-(* TODO: rewrite using a strong specification?  *)
 
 Open Scope bool_scope.
 
@@ -62,29 +62,22 @@ Qed.
 Definition check_eq (eq: equation) (acc: bool*PS.t*PS.t)
                 : bool*PS.t*PS.t :=
   match acc with
-    | (true, defined, variables) =>
-      match eq with
-        | EqDef x ck e =>
-          ((PS.for_all (check_var defined variables)
-                       (free_in_caexp ck e PS.empty))
-             && (negb (PS.mem x defined)),
-           PS.add x defined, PS.add x variables)
-        | EqApp x ck f les =>
-          ((PS.for_all (check_var defined variables)
-                       (free_in_laexps ck les PS.empty))
-             && (negb (PS.mem x defined)),
-           PS.add x defined, PS.add x variables)
-        | EqFby x ck v e =>
-          ((PS.mem x mems && PS.for_all (check_var defined variables)
-                   (free_in_laexp ck e PS.empty))
-             && (negb (PS.mem x defined)),
-           PS.add x defined, variables)
-      end
-    | (false, _, _) => (false, PS.empty, PS.empty)
+  | (true, defined, variables) =>
+    match defined_eq eq with
+    | x => ((PS.for_all (check_var defined variables)
+                        (free_in_equation eq PS.empty))
+              && (negb (PS.mem x defined)),
+            PS.add x defined, add_variable_eq variables eq)
+    end
+  | (false, _, _) => (false, PS.empty, PS.empty)
   end.
 
-Definition well_sch (argIns: Nelist.nelist ident)(eqs: list equation) : bool :=
-  fst (fst (List.fold_right check_eq (true, PS.empty, Nelist.fold_left (fun a b => PS.add b a) argIns PS.empty) eqs)).
+Definition well_sch (args: Nelist.nelist ident) (eqs: list equation) : bool :=
+  fst (fst (List.fold_right check_eq
+                            (true,
+                             PS.empty,
+                             Nelist.fold_left (fun a b => PS.add b a) args PS.empty)
+                            eqs)).
 
 Lemma not_for_all_spec:
   forall (s : PS.t) (f : BinNums.positive -> bool),
@@ -114,173 +107,162 @@ Proof.
   reflexivity.
 Qed.
 
+Lemma in_nelist_fold_left:
+  forall x xs S,
+    PS.In x (Nelist.fold_left (fun S' x => PS.add x S') xs S)
+    <->
+    Nelist.In x xs \/ PS.In x S.
+Proof.
+  induction xs as [|y xs IH].
+  split; intro H; [apply PS.add_spec in H|apply PS.add_spec]; now auto.
+  intro S; split; intro H.
+  - apply IH in H.
+    destruct H.
+    left; apply Nelist.in_necons_spec; auto.
+    apply PS.add_spec in H; simpl; intuition.
+  - simpl; apply IH; simpl in H; intuition.
+Qed.
+
 Lemma well_sch_pre_spec:
-  forall argIns eqs good defined variables,
+  forall args eqs good defined variables,
     (good, defined, variables)
-        = List.fold_right check_eq (true, PS.empty, Nelist.fold_left (fun a b => PS.add b a) argIns PS.empty) eqs
+        = List.fold_right check_eq (true, PS.empty, Nelist.fold_left (fun a b => PS.add b a) args PS.empty) eqs
     ->
     (good = true
-     -> (Is_well_sch mems argIns eqs
+     -> (Is_well_sch mems args eqs
          /\ (forall x, PS.In x defined <-> Is_defined_in_eqs x eqs)
-         /\ (forall x, PS.In x variables <-> Is_variable_in_eqs x eqs \/ Nelist.In x argIns)))
-    /\ (good = false -> ~Is_well_sch mems argIns eqs).
-Admitted. (* XXX: Stating that a decision procedure behaves as expected. Not used *)
-(*
+         /\ (forall x, PS.In x variables <-> Is_variable_in_eqs x eqs \/ Nelist.In x args)))
+    /\ (good = false -> ~Is_well_sch mems args eqs).
+Proof.
   induction eqs as [|eq].
-  - simpl; injection 1; intros HRv HRm; subst.
+  - (* case nil: *)
+    simpl. injection 1. intros.
+    subst variables; subst defined; subst good.
     intuition;
-      repeat match goal with
-               | H: PS.In _ (PS.add _ _) |- _ => rewrite PS.add_spec in H; destruct H
-               | H: PS.In _ PS.empty |- _ => apply PS.empty_spec in H;
-                                             contradiction
-               | H: Is_defined_in _ nil |- _ => now inversion H
-               | H: Is_variable_in _ nil |- _ => now inversion H
-               | H1:good=true, H2:good=false |- _ => rewrite H1 in H2; discriminate
-               | |- _ => tauto
-             end.
-  - intros good defined variables HH.
-    simpl in HH.
-    destruct (List.fold_right check_eq (true, PS.empty, PS.add argIn PS.empty) eqs)
+    repeat match goal with
+           | H:PS.In _ PS.empty |- _ => apply PS.empty_spec in H; contradiction
+           | H:Is_defined_in_eqs _ nil |- _ => inversion H
+           | H:Is_variable_in_eqs _ nil |- _ => inversion H
+           | H: context[Nelist.fold_left _ _ _] |- _ =>
+             apply in_nelist_fold_left in H
+           | _ => intuition
+           end.
+    apply in_nelist_fold_left; auto.
+  - (* case cons: *)
+    intros good defined variables HH.
+    destruct (List.fold_right check_eq (true, PS.empty,
+                 Nelist.fold_left (fun (a : PS.t) (b : positive) => PS.add b a)
+                                  args PS.empty) eqs)
       as [[good' defined'] variables'] eqn:Heq.
     specialize IHeqs with good' defined' variables'.
     pose proof (IHeqs (eq_refl (good', defined', variables'))) as IH;
       clear IHeqs.
     destruct IH as [IHt IHf].
     split; intro Hg; rewrite Hg in *; clear Hg.
-    + destruct eq; (* the horror... *) (* XXX: . was ; *)
-      (simpl in HH;
-       assert (good' = true) as IH
-           by (apply Bool.not_false_iff_true;
-               intro Hgf; rewrite Hgf in HH;
-               discriminate);
-       rewrite IH in HH;
-       apply IHt in IH; clear IHt IHf;
-       destruct IH as [Hwsch [Hidi Hivi]];
-       symmetry in HH;
-       injection HH;
-       intros HRv HRd; rewrite <-HRv,<-HRd in *; clear HRv HRd HH;
-       intro Hcv; apply Bool.andb_true_iff in Hcv;
-         destruct Hcv as [Hcv Hnin];
-         try (apply Bool.andb_true_iff in Hcv;
-               destruct Hcv as [Him Hcv]);
-         rewrite Bool.negb_true_iff,
-         <-PSF.not_mem_iff in Hnin;
-       rewrite PS.for_all_spec in Hcv;
-         [ |now apply check_var_compat];
-       try rewrite PS.mem_spec in Him;
-       split;
-       [constructor;
-         try (exact Hwsch
-              || assumption
-              || (intro HH; apply Hidi in HH; contradiction));
-        intros y Hy;
-          apply free_in_caexp_spec' in Hy
-          || apply free_in_laexp_spec' in Hy;
-          apply Hcv in Hy;
-          apply check_var_spec in Hy;
-          repeat progress match goal with
-          | H:_ /\ _ |- _ => destruct H
-          | |- _ /\ _ => split; intros
-          | H1:PS.In ?y ?mems -> _, H2:PS.In ?y ?mems |- _ => apply H1 in H2
-          | |- ~Is_defined_in ?x _ => intro
-          | H1:~PS.In ?x defined',
-            H2:Is_defined_in ?x eqs |- _ => apply Hidi in H2; contradiction
-          | |- Is_variable_in ?x eqs => auto; apply Hivi
-          | _ => now intuition
-                          end |];
-      (now rewrite <- Hivi; auto) ||
-      split; intro x; split; intro HH;
-         (apply PS.add_spec in HH;
-           destruct HH as [HH|HH]; try (now subst; repeat constructor); [];
-           solve [ now apply Hidi in HH; constructor 2
-                 | apply Hivi in HH; destruct HH as [HH | HH]; tauto || constructor; constructor 2;
-                   []; inversion_clear HH; (now constructor) || (now constructor 2) ])
-         || (rewrite PS.add_spec, ?Hivi, ?Hidi;
-              apply Is_defined_in_cons in HH
-              || (destruct HH as [HH | HH]; try tauto; []; apply Is_variable_in_cons in HH);
-              destruct HH as [HH|HH]; inversion_clear HH; tauto)
-         || (apply Hivi in HH; try (destruct HH as [HH | HH]; tauto || left); constructor 2; apply HH)
-         || (rewrite Hivi; try (destruct HH as [HH | HH]; try tauto; []);
-             apply Is_variable_in_cons in HH; destruct HH as [HH|HH]; inversion HH; tauto)).
-    + destruct good'; [clear IHf| inversion 1; apply IHf; auto ].
-      pose proof (IHt (eq_refl true)) as IH; clear IHt.
-      destruct IH as [Hwsch [Hidi Hivi]].
-      destruct eq;
-        (simpl in HH;
-          injection HH;
-          intros HRd HRv Hcv;
-          rewrite HRd,HRv in *;
-          clear HRd HRv HH;
-          symmetry in Hcv;
-          repeat progress match goal with
-          | Hcv:PS.mem _ _ && _ = false |- _ =>
-            apply Bool.andb_false_iff in Hcv;
-              destruct Hcv as [Hcv|Hcv];
-              [ inversion 1;
-                apply mem_spec_false in Hcv;
-                contradiction
-              | rewrite not_for_all_spec in Hcv;
-                [ |now apply check_var_compat] ]
-          | H:_ && negb _ = false |- _ =>
-            apply Bool.andb_false_iff in Hcv;
-              destruct Hcv as [Hcv|Hcv];
-              [rewrite not_for_all_spec in Hcv;
-                [ |now apply check_var_compat]
-              | rewrite Bool.negb_false_iff in Hcv;
-                rewrite PS.mem_spec in Hcv;
-                apply Hidi in Hcv;
-                inversion 1;
-                contradiction ]
-          | Hcv:PS.mem _ _ && _ && _ = false |- _ =>
-            apply Bool.andb_false_iff in Hcv;
-              destruct Hcv as [Hcv|Hcv];
-              [|rewrite Bool.negb_false_iff in Hcv;
-                 rewrite PS.mem_spec in Hcv;
-                 apply Hidi in Hcv;
-                 inversion 1;
-                 contradiction]
-          | H:PS.for_all _ _ = false |- _ =>
-            apply not_for_all_spec in Hcv; [|apply check_var_compat]
-          | _ => idtac
-          end;
-          intro Hwsch';
-          apply Hcv;
-          inversion_clear Hwsch' as [|? ? ? Hwsch0 HH
-                                        |? ? ? ? Hwsch0 HH
-                                        |? ? ? ? Hwsch0 Hi HH];
-          intros x Hx;
-          apply free_in_caexp_spec in Hx || apply free_in_laexp_spec in Hx;
-          destruct Hx as [Hx|Hx]; [ | apply not_In_empty in Hx; contradiction ];
-          intros;
-          repeat progress
-                 match goal with
-                 | |- _ /\ _ => split; intros
-                 | H: _ /\ _ |- _ => destruct H
-                 | H: Is_free_in_caexp _ _ |- _ => apply HH in H
-                 | H: Is_free_in_laexp _ _ |- _ => apply HH in H
-                 | |- check_var defined' variables' x = true
-                   => apply check_var_spec
-                 | H1:~PS.In ?x ?mems -> Is_variable_in ?x ?eqs,
-                   H2:~PS.In ?x ?mems |- PS.In ?x variables'
-                   => apply H1 in H2; apply Hivi in H2; assumption
-                 | H1:PS.In ?x ?mems -> ~Is_defined_in ?x ?eqs,
-                      H2:PS.In ?x ?mems |- _ => apply H1 in H2
-                 | H:~Is_defined_in ?x ?eqs |- ~PS.In ?x defined'
-                   => intro HN; apply Hidi in HN; contradiction
-                 end);
-          rewrite Hivi; auto.
+    + (* good=true *)
+      simpl in HH; rewrite Heq in HH.
+      simpl in HH.
+      destruct good'; [|discriminate].
+      specialize (IHt eq_refl).
+      clear IHf; destruct IHt as [IHwsch [IHdef IHvar]].
+      injection HH; clear HH; intros Hv Hd H.
+      subst variables; subst defined.
+      symmetry in H.
+      apply Bool.andb_true_iff in H.
+      destruct H as [H1 H2].
+      apply PS.for_all_spec in H1; [|now apply check_var_compat].
+      apply Bool.negb_true_iff in H2.
+      apply mem_spec_false in H2.
+      split; [|split].
+      * (* Is_well_sch *)
+        constructor.
+        assumption.
+        intros x Hfree.
+        apply free_in_equation_spec' in Hfree.
+        apply H1 in Hfree.
+        apply check_var_spec in Hfree.
+        destruct Hfree as [Hfree1 Hfree2].
+        split; intro HH; (apply Hfree1 in HH || apply Hfree2 in HH).
+        intro Hdef; apply IHdef in Hdef; apply HH; assumption.
+        apply IHvar; assumption.
+        intros x Hdef Hdefs; apply IHdef in Hdefs.
+        apply defined_eq_Is_defined_in in Hdef.
+        rewrite Hdef in *.
+        apply H2; assumption.
+      * (* defined set *)
+        intro x; split; intro HH.
+        apply PS.add_spec in HH.
+        destruct HH as [HH|HH].
+        subst x; constructor; apply defined_eq_Is_defined_in; reflexivity.
+        apply IHdef in HH.
+        constructor (assumption).
+        apply PS.add_spec.
+        inversion_clear HH.
+        apply defined_eq_Is_defined_in in H; subst x; auto.
+        right; apply IHdef; assumption.
+      * (* variables set *)
+        intro x; split; intro HH.
+        apply add_variable_eq_empty in HH.
+        destruct HH as [HH|HH].
+        destruct eq;
+          ((apply PS.add_spec in HH;
+             destruct HH as [HH|HH];
+             [subst i; left; now repeat constructor
+             |apply PS.empty_spec in HH; contradiction])
+           || apply PS.empty_spec in HH; contradiction).
+        apply IHvar in HH; intuition; left; constructor (assumption).
+        apply add_variable_eq_empty.
+        destruct HH as [HH|HH].
+        apply Is_variable_in_cons in HH.
+        destruct HH as [HH|HH]; [left|right].
+        destruct eq; inversion_clear HH; simpl; now intuition.
+        apply IHvar; intuition.
+        right; apply IHvar; auto.
+    + (* good=false *)
+      intro Hwsch.
+      simpl in HH; rewrite Heq in HH; clear Heq; simpl in HH.
+      destruct good'; [specialize (IHt eq_refl); clear IHf
+                      | specialize (IHf eq_refl);
+                        apply Is_well_sch_cons in Hwsch;
+                        apply IHf with (1:=Hwsch)].
+      destruct IHt as [_ [IHdef IHvar]].
+      injection HH; clear HH; intros Hv Hd HH.
+      subst variables; subst defined; symmetry in HH.
+      apply Bool.andb_false_iff in HH.
+      inversion_clear Hwsch as [|Ha Hb Hwschs Hfree Hdefd].
+      destruct HH as [HH|HH].
+      * (* check_var of free fails *)
+        apply not_for_all_spec in HH; [|apply check_var_compat].
+        apply HH; clear HH.
+        intros x HH.
+        apply free_in_equation_spec in HH.
+        destruct HH as [HH|HH]; [|apply PS.empty_spec in HH].
+        apply Hfree in HH.
+        destruct HH as [Hmem Hvar];
+          apply check_var_spec; split; intro HHm;
+          (specialize (Hmem HHm) || specialize (Hvar HHm)).
+        intro Hdef; apply IHdef in Hdef; apply Hmem; assumption.
+        apply IHvar; intuition.
+        contradiction.
+      * (* already defined *)
+        apply Bool.negb_false_iff in HH.
+        rewrite PS.mem_spec in HH.
+        apply Hdefd with (i:=defined_eq eq).
+        apply defined_eq_Is_defined_in; reflexivity.
+        apply IHdef; assumption.
 Qed.
-*)
+
 Lemma well_sch_spec:
-  forall argIns eqns,
-    if well_sch argIns eqns
-    then Is_well_sch mems argIns eqns
-    else ~Is_well_sch mems argIns eqns.
+  forall args eqns,
+    if well_sch args eqns
+    then Is_well_sch mems args eqns
+    else ~Is_well_sch mems args eqns.
 Proof.
-  intros argIn eqns.
-  pose proof (well_sch_pre_spec argIn eqns).
+  intros args eqns.
+  pose proof (well_sch_pre_spec args eqns).
   unfold well_sch.
-  destruct (List.fold_right check_eq (true, PS.empty, Nelist.fold_left (fun a b => PS.add b a) argIn PS.empty) eqns)
+  destruct (List.fold_right check_eq
+   (true, PS.empty, Nelist.fold_left (fun a b => PS.add b a) args PS.empty) eqns)
     as [[good defined] variables].
   simpl.
   specialize H with good defined variables.
@@ -288,6 +270,26 @@ Proof.
   destruct H' as [Ht Hf].
   destruct good;
   intuition.
+Qed.
+
+Lemma Is_well_sch_by_refl:
+  forall args eqns, well_sch args eqns = true <-> Is_well_sch mems args eqns.
+Proof.
+  intros args eqns.
+  pose proof (well_sch_spec args eqns) as Hwss.
+  split; intro H.
+  rewrite H in Hwss; assumption.
+  destruct (well_sch args eqns); [reflexivity|].
+  exfalso; apply Hwss; apply H.
+Qed.
+
+Lemma well_sch_dec:
+  forall args eqns,
+    {Is_well_sch mems args eqns}+{~Is_well_sch mems args eqns}.
+Proof.
+  intros args eqns.
+  pose proof (well_sch_spec args eqns) as Hwss.
+  destruct (well_sch args eqns); [left|right]; assumption.
 Qed.
 
 End Decide.
